SSA/Projects/InstCombine/Refinement.lean
@@ -5,7 +5,8 @@ import SSA.Projects.InstCombine.Base
 
 open InstCombine (LLVM)
 
-abbrev Com.Refinement (src tgt : Com LLVM Γ .pure t) (h : TyDenote.toType t = Option α := by rfl) : Prop :=
+abbrev Com.Refinement (src tgt : Com LLVM Γ .pure t)
+    (h : TyDenote.toType t = Option α := by rfl) : Prop :=
   ∀ Γv, (h ▸ src.denote Γv) ⊑ (h ▸ tgt.denote Γv)
 
 infixr:90 " ⊑ "  => Com.Refinement
